\subsection{Exponentialfunktionen}

\paragraph{Allgemeine Form}

\[
	y = a^x \quad a \neq 1
\]

\begin{center}
	\( a > 0 \) damit wir in \( \mathbb{R} \) bleiben

	\( a \) wird Basis genannt, \( x \) Exponent

	\( a > 1 \) monoton steigend

	\( a < 1 \) monoton fallend
\end{center}

\begin{figure}[H]
	\centering
	\begin{tikzpicture}
		\begin{axis}[
				defaultnonumbers,
				xmin=-2.2, xmax=2.2,
				ymin=-1.2, ymax=3.2,
				width=8cm
			]
			\addplot[orange, smooth, samples=100, domain=-4:4] {e^x};
			\addplot[cyan, smooth, samples=100, domain=-4:4] {e^-x};
			\node [right] at (axis cs: 1.2, 3) {\( a > 1 \)};
			\node [left] at (axis cs: -1.2, 3) {\( a < 1 \)};
		\end{axis}
	\end{tikzpicture}
	\caption{exponentiell steigend (\( e^x \)) und fallend (\( e^{-x} \))}
\end{figure}

\begin{figure}[H]
	\centering
	\begin{align*}
		y(t)        & = {(1 + \omega)}^{t} \cdot y_0                            \\
		\Delta y(t) & \sim y(t-1)                                               \\
		\Delta y(t) & = \omega \cdot y(t-1) \quad \omega : \text{Wachstumsrate}
	\end{align*}
	\begin{tikzpicture}
		\begin{axis}[
				default,
				xmin=-1.2, xmax=6.2,
				ymin=-0.2, ymax=5.2,
				width=10cm,
				height=12cm,
				yticklabels={},
				xlabel={t},
			]
			\addplot [orange, smooth, samples=100, domain=-4:4] {e^(0.5*x)};

			\node [left] at (axis cs: -0.2, 1.0000) {\( y(0) \)};
			\node [left] at (axis cs: -0.2, 1.6487) {\( y(1) \)};
			\node [left] at (axis cs: -0.2, 2.7183) {\( y(2) \)};
			\node [left] at (axis cs: -0.2, 4.4817) {\( y(3) \)};

			\draw [dotted, thick] (-0.2, 1.0000) -- (6.2, 1);
			\draw [dotted, thick] (-0.2, 1.6487) -- (6.2, 1.6487);
			\draw [dotted, thick] (-0.2, 2.7183) -- (6.2, 2.7183);
			\draw [dotted, thick] (-0.2, 4.4817) -- (6.2, 4.4817);

			\draw [decorate,decoration={brace,amplitude=4pt}] (1, 1.6487) -- (1, 1);
			\draw [decorate,decoration={brace,amplitude=4pt}] (2, 2.7183) -- (2, 1.6487);
			\draw [decorate,decoration={brace,amplitude=4pt}] (3, 4.4817) -- (3, 2.7183);

			\node [right] at (axis cs: 1.2, 1.3244) {\( \Delta y(1) = \omega \cdot y(0) \)};
			\node [right] at (axis cs: 2.2, 2.1835) {\( \Delta y(2) = \omega \cdot y(1) \)};
			\node [right] at (axis cs: 3.2, 3.6000) {\( \Delta y(3) = \omega \cdot y(2) \)};
		\end{axis}
	\end{tikzpicture}
	\[
		\begin{alignedat}{5}
			\Delta y(3) &= y(3) - y(2) &= \omega \cdot y(2) \quad
			&\Rightarrow y(3) &= y(2) \cdot (1 + \omega) &= y(0) \cdot {(1+\omega)}^3 \\
			\Delta y(2) &= y(2) - y(1) &= \omega \cdot y(1) \quad
			&\Rightarrow y(2) &= y(1) \cdot (1 + \omega) &= y(0) \cdot {(1+\omega)}^2 \\
			\Delta y(1) &= y(1) - y(0) &= \omega \cdot y(0) \quad
			&\Rightarrow y(1) &= y(0) \cdot (1 + \omega) &= y(0) \cdot (1+\omega)
		\end{alignedat}
	\]
	% \caption{}
\end{figure}

\begin{uebung}[1]
	\begin{equation*}
		\begin{array}{lrl}
			                & 9^{x-1}       & = 27          \\
			\Leftrightarrow & 9^{x-1}       & = 3^3         \\
			\Leftrightarrow & {(3^2)}^{x-1} & = 3^3         \\
			\Leftrightarrow & 3^{2x-2}      & = 3^3         \\
			\Rightarrow     & 2x-2          & = 3           \\
			\Leftrightarrow & 2x            & = 5           \\
			\Leftrightarrow & x             & = \frac{5}{2}
		\end{array}
	\end{equation*}
\end{uebung}

\begin{uebung}[2]
	\begin{equation*}
		\begin{array}{lrl}
			                & {\left(\frac{4}{9}\right)}^{x-2}                    & = \frac{8}{27} \\
			\Leftrightarrow & {\left(\frac{4}{9}\right)}^{x-2}                    & =
			{\left(\frac{2}{3}\right)}^{3}                                                         \\
			\Leftrightarrow & {\left({\left(\frac{2}{3}\right)}^{2}\right)}^{x-2} & =
			{\left(\frac{2}{3}\right)}^{3}                                                         \\
			\Leftrightarrow & {\left(\frac{2}{3}\right)}^{2x-4}                   & =
			{\left(\frac{2}{3}\right)}^{3}                                                         \\
			\Rightarrow     & 2x-4                                                & = 3            \\
			\Leftrightarrow & 2x                                                  & = 7            \\
			\Leftrightarrow & x                                                   & = \frac{7}{2}
		\end{array}
	\end{equation*}
\end{uebung}

\begin{uebung}[3]
	\begin{equation*}
		\begin{array}{lrlr}
			                & 8 \cdot 9^{x-3} + 4^{x-3}     & = 3^{2x-4}                                    &                            \\
			\Leftrightarrow & 8 \cdot 3^{2x-9} + 4^{x-3}    & = 3^{2x-4}                                    &                            \\
			\Leftrightarrow & 2^3 \cdot 3^{2x-9} + 2^{2x-6} & = 3^{2x-4}                                    & \mid -(2^3 \cdot 3^{2x-9}) \\
			\Leftrightarrow & 2^{2x-6}                      & = 3^{2x-4} - 2^3 \cdot 3^{2x-9}               &                            \\
			\Leftrightarrow & 2^{2x-6}                      & = 3^{2} \cdot 3^{2x-6} - 2^{3} \cdot 3^{2x-9}                              \\
			\Leftrightarrow & 2^{2x-6}                      & = (3^2 - 2^3)
			% TODO: siehe Zettel - ergÃ¤nzen 
		\end{array}
	\end{equation*}
\end{uebung}
