\subsection{Potentielle Ableitungen}

% TODO: 3D-Graph

\begin{align*}
    y' &= \frac{\diff y}{\diff x} \\
    y'' &= \frac{\diff^2 y}{\diff x^2} \\
    \\
    \frac{\partial f}{\partial x} &= f_x \qquad f_y \\
    \frac{\partial^2 f}{\partial x^2} &= 
    \begin{array}{ll}
        f_{xx} & f_{yx} \\
        f_{xy} & f_{yy}
    \end{array} \\
    \\
    f_{yxy} &= f_{xyy} = f_{yyx}
\end{align*}

\begin{align*}
    z &= f(x, y) = e^{x^2 + y^2} \\
    f_x &= \left( x^2 + y^2 \right)' = e^{x^2 + y^2} \cdot 2 x
    &f_{xy} = 2y \cdot e^{x^2 + y^2} \cdot 2x \\
    f_y &= \left( e^{x^2 + y^2} \right)' = e^{x^2 + y^2} \cdot 2 y
    &f_{yx} = 2x \cdot e^{x^2 + y^2} \cdot 2y
\end{align*}

\paragraph{Ãœbungen}

\subparagraph{1)}

\begin{align*}
    f(x, y) &= a^x \cdot y^a \\
    f_x &= a^x \cdot \ln a \cdot y^a \\
    f_y &= a^x \cdot a \cdot y^{a-1} \\
    &= a^{x+1} \cdot y^{a-1}
\end{align*}

\subparagraph{2)}

\begin{align*}
    f(x, y) &= e^{x y} \cdot \frac{x}{y} \\
    f_x &= e^{x y} \cdot \frac{1}{y} + e^{x y} \cdot y \cdot \frac{x}{y} \\
    &= e^{x y} \left( \frac{1}{y} + x \right) \\
    f_y &= \frac{x}{y} \cdot e^{x y} \cdot x + e^{x y} \left(-x y^{-2} \right) \\
    &= e^{x y} \left( \frac{x^2}{y} - \frac{x}{y^2} \right) \\
    f_{xy} &= e^{x y} \cdot x \left( \frac{1}{y} + x \right) + e^{x y} \left( - \frac{1}{y^2} \right) \\
    &= e^{x y} \left( \frac{x}{y} + x^2 - \frac{1}{y^2} \right)
\end{align*}
