\subsection{Gau√üscher Algorithmus}

\begin{align*}
	\sum_{i=1}^n a_i         & = a_1 + a_2 + a_3 + \cdots + a_{n-1} + a_n                         \\
	\\
	\sum_{i=1}^n a_i         & = a + (a + d) + (a + 2d) + \cdots + (a +(n-2) d) + (a + (n - 1) d) \\
	\sum_{i=1}^n a_i         & = (a + (n-1)d) + (a +(n-2) d) + \cdots + (a + 2d) + (a + d) + a    \\
	\cline{1-2}
	2 \cdot \sum_{i=1}^n a_i & = (2a+(n-1)d) + (2a+(n-1)d) + \cdots + (2a+(n-1)d)                 \\
	\\
	2 \cdot \sum_{i=1}^n a_i & = n (2a+(n-1)d) = 2n a + n(n-1)d
\end{align*}

\begin{gesetz}
	\paragraph{Summe einer arithmetischen Folge bis \(n\)}
	\[
		\sum_{i=1}^n a_i = n a + \frac{n(n-1)}{2} d
	\]
\end{gesetz}
