\subsection{Aufgaben}

\paragraph{1)}

\begin{align*}
    \int_4^5 \frac{x^2}{x-2} \;\mathrm{d}x \\
    &= \int_4^5 x+3 + \frac{9}{x-3} \;\mathrm{d}x \\
    &= \int_4^5 x \;\mathrm{d}x + 3 \int_4^5 1 \;\mathrm{d}x + 9 \int_4^5 \frac{1}{x-3} \;\mathrm{d}x \\
    &= {\left[ \frac{x^2}{2} \right]}_4^5 + 3 {[x]}_4^5 + 9 {[\ln (x-3)]}_4^5 \\
    &= {\left[ \frac{x^2}{2} + 3x + 9 \cdot \ln(x-3) \right]}_4^5 \\
    &= \frac{25}{2} + 15 + 9 \cdot \ln(2) - \frac{16}{2} - 12 -9 \cdot \ln(1) \\
    &= \frac{15}{2} + 9 \ln(2) \approx 13,74\;\mathrm{FE}
\end{align*}

% TODO: Nebenrechnung auch layoutmäßig daneben

\subparagraph{Nebenrechnung}

\polyset{style=C, div=:,vars=x}
\polylongdiv{x^2}{x-3}

\paragraph{2)}

\begin{align*}
    &u(x) = \sin(x) \\
    \\
    I)\quad &\frac{\mathrm{d}u}{\mathrm{x}} = \cos(x) \Rightarrow \mathrm{d}x = \frac{\mathrm{d}u}{\cos(x)} \\
    &u(\frac{\pi}{2}) = 1; U(0) = 0 \\
    &\int_0^1 u^4 \cdot \cos(x) \cdot \frac{\mathrm{d}u}{\cos(x)} \\
    &= {\left[ \frac{u^5}{5} \right]}_0^1 = \frac{1}{5} \\
    II)\quad &u = \sin^4(x) \Rightarrow u' = 4 \sin^3 (x) \\
    &v' = \cos(x) \Rightarrow v = \sin(x) \\
    &\Rightarrow = {\left[ \sin^5(x) \right]}_0^{\frac{\pi}{2}} - 4 \int_0^{\frac{\pi}{2}} \sin^4 (x) \cdot \cos(x) \\
    &\Rightarrow 5 \int_0^\frac{\pi}{2} \sin^4(x) \cdot \cos(x) \;\mathrm{d}x = {\left[ \sin^5(x) \right]}_0^\frac{0}{\frac{\pi}{2}} \\
    &\Rightarrow \int_0^\pi \sin^4(x) \cdot \cos(x) \;\mathrm{d}x = \frac{1}{5} {\left[ \sin^5(x) \right]}_0^\frac{\pi}{2} \\
    &= \frac{1}{5}
\end{align*}

\paragraph{3)}

\begin{align*}
    &\int \frac{1}{x} \cdot \ln(x) \;\mathrm{d}x \\
    \\
    &\begin{array}{ll}
        u = \ln x &\Rightarrow u'= \frac{1}{x} \\
        v' = \frac{1}{x} &\Rightarrow v = \ln x 
    \end{array} \\
    &\Rightarrow{} \ln^2 x- \int\frac{1}{x} \cdot \ln(x) \;\mathrm{d}x = \frac{1}{x} \ln(x) \;\mathrm{d}x \\
    &\Rightarrow{} 2 \cdot \int\frac{1}{x} \ln(x) \;\mathrm{d}x = \ln^2(x) \\
    &\int\frac{1}{x} \ln(x) \;\mathrm{d}x = \frac{1}{2} \ln^2 (x) + C
\end{align*}

\paragraph{4)}

\begin{align*}
    &\int \frac{1-x}{1+\sqrt{x}} \;\mathrm{d}x = \int \frac{1^2 - \sqrt{2}}{1+ \sqrt{x}} \;\mathrm{d}x \\
    \\
    &\Rightarrow = \int \frac{(1 + \sqrt(x) (1 - \sqrt{x}))}{1 + \sqrt{x}} \\
    &= \int 1 - \sqrt{x} \;\mathrm{d}x \\
    &= \int \;\mathrm{d}x - \int \sqrt{x} \;\mathrm{d}x \\
    &= x - \frac{2}{3} x^{\frac{3}{2}} + C     
\end{align*}

\paragraph{5)}

\begin{align*}
    &\int \ln(x) \;\mathrm{d}x \\
    \\
    &= \int \ln(x) \cdot 1 \;\mathrm{d}x \\
    &\begin{array}{ll}
        u = \ln(x) &\Rightarrow u' = \frac{1}{x} \\
        v' = 1 &\Rightarrow v = x
    \end{array} \\
    &\Rightarrow\int\ln(x) \;\mathrm{d}x \\
    &= \ln(x) \cdot x- \int\frac{1}{x} x \;\mathrm{d}x \\
    &= \ln(x) x-x+C \\
    &= x (\ln(x)-1) +C
\end{align*}

\paragraph{6)}

\begin{align*}
    &\int \frac{1}{x \cdot \ln x} \;\mathrm{d}x \\
    \\
    &z = \ln (x) \\
    &\frac{\mathrm{d} z}{\mathrm{d} x} = \frac{1}{x} \Rightarrow \mathrm{d} x = x \cdot \mathrm{d} z \\
    &= \int \frac{1}{x} \frac{1}{z} x \mathrm{d}z \\
    &= \int \frac{1}{z} \mathrm{d} z \\
    &= \ln|z| + C \\
    &= \ln|\ln|x|| + C
\end{align*}
