\subsection{Rechenregeln}

\begin{gesetz}
    \begin{alignat*}{3}
        \text{1.}\quad & \int_a^b u \cdot f(x) \,\mathrm{d}x &&= u \cdot \int_a^b f(x) \,\mathrm{d}x \\
        \text{2.}\quad & \int_a^b \left( f(x) + g(x) \right) \,\mathrm{d}x &&= \int_a^b f(x) \,\mathrm{d}x + \int_a^b g(x) \,\mathrm{d}x \\
        \text{3.}\quad & \int_a^b f(x) \,\mathrm{d}x &&= -\int_b^a f(x) \,\mathrm{d}x \\
        \text{4.}\quad & \int_a^a f(x) \,\mathrm{d}x &&= 0 \\
        \text{5.}\quad & \int_a^c f(x) \,\mathrm{d}x &&= \int_a^b f(x) \,\mathrm{d}x + \int_b^c f(x) \,\mathrm{d}x
    \end{alignat*}
\end{gesetz}
