\subsection{Ãœbungen}

\paragraph{1)}

\begin{align*}
    \int (x^2 + 2x - 5) \;\mathrm{d}x \\
    &= \int x^2 \;\mathrm{d}x + \int 2x \;\mathrm{d}x - 5 \int \;\mathrm{d}x \\
    &= \frac{x^3}{3} + 2 \frac{x^2}{2} - 5x + C \\
    &= \frac{x^3}{3} + x^2 - 5x + C
\end{align*}

\paragraph{2)}

\begin{align*}
    \int \frac{x^2 - 8x}{x^4} \;\mathrm{d}x;
    &= \int \frac{x^2}{x^4} \;\mathrm{d}x - \int \frac{8x}{x^4} \;\mathrm{d}x \\
    &= \int x^{-2} \;\mathrm{d}x - 8 \int x^{-3} \;\mathrm{d}x \\
    &= \frac{x^{-1}}{-1} - 8 \frac{x^{-2}}{-2} + C \\
    &= -\frac{1}{x} + 4 \frac{1}{x^2} + C
\end{align*}

\paragraph{3)}

\begin{align*}
    \int_2^3 \frac{x-3}{x^2} \;\mathrm{d}x \\
    &= \int_2^3 \frac{1}{x} \;\mathrm{d}x - 3 \int_2^3 \frac{1}{x^2} \;\mathrm{d}x \\
    &= {[\ln x]}_2^3 - 3 {\left[- \frac{1}{x}\right]}_2^3 \\
    &= \ln 3 - \ln 2 + 3 {\left[\frac{1}{x}\right]}_2^3 \\
    &= \ln \frac{3}{2} + \left(\frac{3}{3} - \frac{3}{2}\right) \\
    &= \ln \frac{3}{2} - \frac{1}{2} \\
    &\approx -0.095
\end{align*}

\paragraph{4)}

\begin{align*}
    \int \frac{x-5}{x^2 - x - 6} \;\mathrm{d}x \\
    &= \int \frac{x-5}{(x+2)(x-3)} \;\mathrm{d}x \\
    \text{NR:\;Partialbruchzerlegung} \\
    \frac{x-5}{(x+2)(x-3)} &= \frac{A}{x+2} + \frac{B}{x-3} \\
    x-5 &= A(x-3) + B(x+2) \\
    x=-2:\quad -7 &= -5A \Rightarrow A = \frac{7}{5} \\
    x=3:\quad -2 &= 5B \Rightarrow B = -\frac{2}{5} \\
    \Rightarrow &= \frac{7}{5} \int \frac{1}{x+2} \;\mathrm{d}x - \frac{2}{5} \int \frac{1}{x-3} \;\mathrm{d}x
\end{align*}


\begin{alignat*}{2}
    \text{Substitutionsmethode} \\
    \text{1.)}\quad &\int \frac{1}{x+2} \;\mathrm{d}x \,\text{mit}\, z &&= x + 2 \\
    &\int \frac{1}{z} \;\mathrm{d}x &&= \;\mathrm{d}z \\
    &\int \frac{1}{2} \;\mathrm{d}z = \ln z &&= \ln (x + 2) \\
    \text{2.)}\quad &\int \frac{1}{x-3} \;\mathrm{d}x \,\text{mit}\, y &&= x - 3 \\
    &\int \frac{1}{y} \;\mathrm{d}x \;\mathrm{d}x &&= \;\mathrm{d}y \\
    &\int \frac{1}{y} \;\mathrm{d}y = \ln y &&= \ln(x-3)
\end{alignat*}

\[
    \Rightarrow = \frac{7}{5} \ln(x+2) - \frac{2}{5} \ln(x-3) + C 
\]
    