\subsection{Trigonometrische Reihen}

\begin{align*}
	f(x)      & =\sin x  & f(0)      & =0     & f(x)      & = \cos x  & f(0)      & = 1    \\
	f'(x)     & =\cos x  & f'(0)     & =1     & f'(x)     & = -\sin x & f'(0)     & = 0    \\
	f''(x)    & =-\sin x & f''(0)    & =0     & f''(x)    & = -\cos x & f''(0)    & = -1   \\
	f'''(x)   & =-\cos x & f'''(0)   & =-1    & f'''(x)   & = \sin x  & f'''(0)   & = 0    \\
	f^{IV}(x) & =\sin x  & f^{IV}(0) & =0     & f^{IV}(x) & = \cos x  & f^{IV}(0) & = 1    \\
	          & \vdots   &           & \vdots &           & \vdots    &           & \vdots
\end{align*}

\[
	\sin x = x - \frac{x^3}{3!} + \frac{x^5}{5!} - \frac{x^7}{7!} + \ldots \qquad
	\cos x = 1 - \frac{x^2}{2!} + \frac{x^4}{4!} - \frac{x^6}{6!} + \ldots
\]

\subsubsection{Eulergleichung}

\begin{align*}
	e^{\mathrm{i}x} & = \cos x + \mathrm{i} \cdot \sin x                                                                                                                                       \\
	e^x             & = 1 + \frac{x}{1!} + \frac{x^2}{2!} + \frac{x^3}{3!} + \frac{x^4}{4!}  + \frac{x^5}{5!} + \ldots                                                                         \\
	e^{\mathrm{i}x} & = 1 + \mathrm{i} x - \frac{x^2}{2!} - \mathrm{i} \frac{x^3}{3!} + \frac{x^4}{4!} \pm \ldots                                                                              \\
	                & = \left( 1 - \frac{x^2}{2!} + \frac{x^4}{4!} + \frac{x^6}{6!} + \ldots \right) + \mathrm{i} \left( x - \frac{x^3}{3!} + \frac{x^5}{5!} - \frac{x^7}{7!} + \ldots \right) \\
	                & = \cos x + \mathrm{i} \cdot \sin x
\end{align*}

\begin{gesetz}
	\[
		1 \cdot e^{\mathrm{i} \pi} = -1
	\]
\end{gesetz}
