\subsection{Ableitungsregeln}

\begin{enumerate}
	\item Konstantenregel
	      \begin{align*}
		      y(x)  & = c \\
		      y'(x) & = 0
	      \end{align*}
	\item Faktorregel
	      \begin{align*}
		      y(x)  & = c \cdot u(x)  \\
		      y'(x) & = c \cdot u'(x)
	      \end{align*}
	\item Summenregel
	      \begin{align*}
		      y(x)  & = u(x) + v(x)   \\
		      y'(x) & = u'(x) + v'(x)
	      \end{align*}
	\item Produktregel
	      \begin{align*}
		      y(x)  & = u(x) \cdot v(x)                     \\
		      y'(x) & = u(x) \cdot v'(x) + u'(x) \cdot v(x)
	      \end{align*}
	\item Quotientenregel
	      \begin{align*}
		      y(x)  & = \dfrac{u(x)}{v(x)}                                  \\
		      y'(x) & = \dfrac{v(x) \cdot u'(x) - v'(x) \cdot u(x)}{v^2(x)}
	      \end{align*}
	\item Kettenregel
	      \begin{align*}
		      y(x)  & = f(\phi(x)) = f(z),\ z = \phi(x)                                                                                                                           \\
		      y'(x) & = \dfrac{\diff y}{\diff x} = \underbrace{\dfrac{\diff f}{\diff z}}_{\text{äußere Abl.}} \cdot \underbrace{\dfrac{\diff \phi}{\diff x}}_{\text{innere Abl.}}
	      \end{align*}
	\item Ableitung der Umkehrfunktion
	      \begin{align*}
		      f(x)  & = y,\ x = f^{-1}(f(x))                \\
		      f'(x) & = \dfrac{1}{\dfrac{\diff f}{\diff x}}
	      \end{align*}
	\item Logarithmisches Differenzieren
	      \begin{align*}
		      y(x) & = u{(x)}^{v(x)}                            \\
		           & \text{I.\, logarithmiere}                  \\
		           & \text{II.\, differenzieren mit Regel 1--7}
	      \end{align*}
\end{enumerate}
