\subsubsection{Beispiel Kurvendiskussion}

\[
	y = f(x) = \frac{x^3 - 2x^2}{x^2 - x - 2} = x^2 \frac{x - 2}{x^2 - x - 2} = x^2 \frac{x - 2}{(x-2)(x+1)}
\]

\paragraph{Definitionsbereich}

\begin{align*}
	x^2 - x - 2 & = 0                                                        \\
	x_{P1,2}    & = \frac{1}{2} \pm \sqrt{\frac{1}{4} + \frac{8}{4}}         \\
	x_{P1}      & = -1,\quad x_{P2} = 2                                      \\
	D_f         & = \{ x \in \mathbb{R}\ |\ (x \neq -1) \wedge (x \neq 2) \}
\end{align*}

\subparagraph{Ersatzfunktionen}

\begin{align*}
	y* = x^2 \frac{\cancel{x - 2}}{\cancel{(x - 2)}(x + 1)} = \frac{x^2}{x + 1}
\end{align*}

\paragraph{Nullstellen}

\begin{align*}
	x_{N1,2} & = 0 \\
	x_{N3}   & = 2
\end{align*}

\paragraph{Verhalten im Fernbereich}

\begin{alignat*}{2}
	\limfromto{x}{-1_+} f(x) & = \frac{x^2}{x + 1} & = +\infty \\
	\limfromto{x}{-1_-} f(x) & = \frac{x^2}{x + 1} & = -\infty
\end{alignat*}

\paragraph{Asymptote}

\polyset{style=C, div=:,vars=x}
\polylongdiv{x^2}{x + 1}

\[
	y_A = x - 1 \qquad y^A = x - 1 + \frac{1}{x + 1}
\]

\paragraph{Ableitung}

\begin{align*}
	(y*)' & = \frac{(x + 1) 2x - x^2}{{(x + 1)}^2}
	= \frac{2x^2 + 2x - x^2}{{(x + 1)}^2}
	= \frac{x^2 + 2x}{{(x + 1)}^2}
	= x \frac{x + 2}{{(x + 1)}^2}
\end{align*}

\[
	\begin{array}{cccc}
		x_{E1} = 0  & y_{E1} = 0  & y_A''(x_{E1}) > 0 \Rightarrow \text{Minimum} \\
		x_{E2} = -2 & y_{E2} = -4 & y_A''(x_{E2}) < 0 \Rightarrow \text{Maximum}
	\end{array}
\]

\begin{align*}
	y^A     & = x - 1 + \frac{1}{x + 1}            \\
	(y^A)'  & = 1 - \frac{1}{{(x + 1)}^2}          \\
	        & = 1 - {(x + 1)}^{-2}                 \\
	(y^A)'' & = 2{(x + 1)}^{-3}                    \\
	        & = \frac{2}{{(x + 1)}^3}              \\
	        & \Rightarrow \text{Keine Wendestelle}
\end{align*}

\paragraph{Zeichnung}

\begin{figure}[H]
	\centering
	\begin{tikzpicture}
		\begin{axis}[
				default,
				xmin=-8.5, xmax=8.5,
				ymin=-8.5, ymax=8.5,
				width=12cm,
			]

			\addplot[color1, smooth, samples=100, domain=2.1:8] {(x^3 - 2*x^2)/(x^2 - x -2)};

			\addplot[color1, smooth, samples=100, domain=-1:1.9] {(x^3 - 2*x^2)/(x^2 - x -2)};

			\addplot[color1, smooth, samples=100, domain=-8:-1.1] {(x^3 - 2*x^2)/(x^2 - x -2)};

			\addplot[color3, dashed, smooth, samples=100, domain=-8:8] {x-1};

			\draw[color2, dotted, thick] (-1, -9) -- (-1, 9);

			\draw[color2, dotted, thick] (2, -9) -- (2, 9);
		\end{axis}
	\end{tikzpicture}
	\caption{Skizze}
\end{figure}
